Finite sets are now restricted to representative without duplicates.
This will simplify computions of cardinals and other interpretations in commutative monoids (or more generally traversals by commutative applicatives). It will also be useful when finite functions come around.

FinSet.v
@@ -6,20 +6,39 @@ Require Coq.Setoids.Setoid.
 Require Import Coq.Classes.RelationClasses.
 Require Import Coq.Classes.Morphisms.
 Require Import FinSet.Lib.ListSet.
+Require Import FinSet.Quotients.UList.
 Require Import FinSet.Lib.DProp.
 Require Import FinSet.Quotients.Countable.
 Require Import FinSet.Quotients.Retract.
 Require Import FinSet.Quotients.Quotient.
 
 
-Definition T (A:Type) {_:Countable A} : Type := Quotient (eq_set_list eq_countable).
-
-Definition listset {A} {_:Countable A} :=
-  (quotient (eq_set_list eq_countable)).
+Definition T (A:Type) {_:Countable A} : Type := Quotient (eq_set_ulist eq_countable).
 
 Instance set_countable (A:Type) {_:Countable A} : Countable (T A).
 Proof. typeclasses eauto. Defined.
 
+(** * Low level interface *)
+
+Definition listset {A} {_:Countable A} : Retract (list A) (T A) :=
+  Retract.compose ulist (quotient (eq_set_ulist eq_countable)).
+
+Lemma set_quotient A (_:Countable A) : forall x,
+  eq_set_list eq_countable (listset.(inj) (listset.(proj) x)) x.
+Proof.
+  intros x. unfold listset,compose. cbn [inj proj].
+  rewrite Quotient.universal.
+  apply ulist_eq_set.
+  { typeclasses eauto. }
+Qed.
+
+Lemma set_unique A (_:Countable A) :
+  forall x, nodup eq_countable (listset.(inj) x).
+Proof.
+  intros x. unfold listset,compose. cbn [inj].
+  apply ulist_nodup.
+Qed.
+  
 
 (** * Quantifiers *)
 
@@ -115,7 +134,7 @@ Section SetOperations.
  Lemma empty_spec : forall x, ~x∈empty.
  Proof.
    intros x n. unfold empty in n.
-   rewrite mem_spec, Quotient.universal in n.
+   rewrite mem_spec, set_quotient in n.
    eauto.
  Qed.
 
@@ -131,7 +150,7 @@ Section SetOperations.
 
  Lemma singleton_spec : forall x a, x∈(singleton a) <-> x=a.
  Proof.
-   intros *. unfold singleton. rewrite mem_spec_in, Quotient.universal.
+   intros *. unfold singleton. rewrite mem_spec_in, set_quotient.
    cbn. intuition.
  Qed.
 
@@ -146,7 +165,7 @@ Section SetOperations.
  Lemma union_spec : forall x u₁ u₂, x∈(union u₁ u₂) <-> x∈u₁ \/ x∈u₂.
  Proof.
    intros *. unfold union.
-   rewrite mem_spec,Quotient.universal.
+   rewrite mem_spec,set_quotient.
    rewrite mem_list_app. unfold mem.
    reflexivity.
  Qed.
@@ -159,7 +178,7 @@ Section SetOperations.
 
  Lemma Union_spec u F x : x ∈ (Union u F) <-> exists y, y∈u /\ x ∈ (F y).
  Proof.
-   unfold Union. rewrite mem_spec_in,  Quotient.universal.
+   unfold Union. rewrite mem_spec_in,  set_quotient.
    rewrite List.in_flat_map.
    split.
    + intros [a [ha₁ ha₂]]. eexists.
@@ -194,7 +213,7 @@ Lemma guard_spec_tt P : tt∈(guard P) <-> P.
 Proof.
   unfold guard.
   destruct (dec P) as [p|n].
-  + rewrite mem_spec, Quotient.universal.
+  + rewrite mem_spec, set_quotient.
     ddecide (mem_list eq_countable tt [tt]) h. cbn.
     intuition.
   + generalize (empty_spec _ _ tt).
